theories/Fresh.v
@@ -1,19 +1,23 @@
 From Nominal Require Import Nominal.
 
-Record freshT `{Nominal X} (a : name) (x : X) : Type := mkFreshT {
-  new : name;
-  new_fresh : new ∉ support x;
-  new_fixpoint : ⟨a,new⟩ • x ≡@{X} x
-}.
+(* Record freshT `{Nominal X} (a: name) (x: X): Type := mkFreshT {
+  new: name;
+  new_fresh: new ∉ support x;
+  new_fixpoint: ⟨a,new⟩ • x ≡@{X} x
+}. *)
 
 Definition freshP_e `{Nominal X} (a: name) (x: X) := ∃ (b : name), b ∉ support x ∧ ⟨a,b⟩ • x ≡@{X} x.
 Definition freshP_a `{Nominal X} (a: name) (x: X) := ∀ (b : name), b ∉ support x → ⟨a,b⟩ • x ≡@{X} x.
 
-Infix "#" := freshT (at level 50).
-Infix "#ₚₑ" := freshP_e (at level 50).
-Infix "#ₚₐ" := freshP_a (at level 50).
+(* Infix "#" := freshT (at level 50). *)
+(* Infix "#ₚₑ" := freshP_e (at level 50). *)
+Infix "#" := freshP_e (at level 50).
+Notation "a #( x , y )" := (a # x ∧ a # y) (at level 50).
+Notation "a #( x , y , z )" := (a # x ∧ a # y ∧ a # z) (at level 50).
+Notation "a #( x , y , z , w )" := (a # x ∧ a # y ∧ a # z ∧ a # w) (at level 50).
+Infix "#ₐ" := freshP_a (at level 50).
 
-Lemma some_any `{Nominal X} (a: name) (x: X) : a #ₚₑ x ↔ a #ₚₐ x.
+Lemma some_any_iff `{Nominal X} (a: name) (x: X) : a # x ↔ a #ₐ x.
 Proof.
   split.
   - intros [b [SB HH]] c SC; destruct (decide (c = a)), (decide (c = b)); subst; auto.
@@ -24,38 +28,39 @@ Proof.
     + apply HH, is_fresh.
 Qed.
 
-Lemma fresh_spec_el `{Nominal X} (a: name) (x: X) : a # x → a #ₚₑ x.
-Proof. intros [n ? ?]; exists n; split; auto. Qed.
+(* Lemma fresh_spec_el `{Nominal X} (a: name) (x: X) : a # x → a #ₚₑ x.
+Proof. intros [n ? ?]; exists n; split; auto. Qed. *)
 
-Lemma fresh_spec_al `{Nominal X} (a: name) (x: X) : a # x → a #ₚₐ x.
-Proof. intro; apply some_any, fresh_spec_el; auto. Qed.
+(* Lemma fresh_spec_al `{Nominal X} (a: name) (x: X) : a # x → a #ₚₐ x.
+Proof. intro; apply some_any, fresh_spec_el; auto. Qed. *)
 
-Definition fresh_spec_ar `{Nominal X} (a: name) (x: X) : a #ₚₐ x → a # x.
+(* Definition fresh_spec_ar `{Nominal X} (a: name) (x: X) : a #ₚₐ x → a # x.
 Proof. 
   intros HH; constructor 1 with (fresh (support x)); pose proof (is_fresh (support x));
     specialize (HH (fresh (support x)) H1); auto.
-Defined.
+Defined. *)
 
-Definition fresh_spec_er `{Nominal X} (a: name) (x: X) : a #ₚₑ x → a # x.
-Proof. intros HH; apply fresh_spec_ar, some_any; assumption. Defined.
+(* Definition fresh_spec_er `{Nominal X} (a: name) (x: X) : a #ₚₑ x → a # x.
+Proof. intros HH; apply fresh_spec_ar, some_any; assumption. Defined. *)
 
 Lemma support_fresh `{Nominal X} (a : name) (x: X): a ∉ support x → a # x.
-Proof. intros; econstructor; [idtac | eapply perm_action_equal]; auto. Qed.
+Proof. intros; econstructor; split; [idtac | eapply perm_action_equal]; assumption. Qed.
 
-Definition update_fresh `{Nominal X} (a b: name) (x: X) : a # x → b ∉ support x → a # x.
-Proof. intros F ?; eapply fresh_spec_al in F; unfold freshP_a in F; econstructor; eauto. Defined. 
+(* Pode ser importante na frente *)
+(* Definition update_fresh `{Nominal X} (a b: name) (x: X): a # x → b ∉ support x → a # x.
+Proof. intros F ?; eapply fresh_spec_al in F; unfold freshP_a in F; econstructor; eauto. Defined.  *)
 
 (* Lemma support_fresh_a `{Nominal X} (a : name) (x: X): a ∉ support x → a #ₐ x.
 Proof. intros; apply some_any, support_fresh_e; auto. Qed. *)
 
 Lemma fresh_support_fresh `{Nominal X} (x: X): fresh (support x) # x.
-Proof. constructor 1 with (fresh (support x)); [apply is_fresh | apply perm_action_equal]. Qed.
+Proof. constructor 1 with (fresh (support x)); split; [apply is_fresh | apply perm_action_equal]. Qed.
 
 Lemma fresh_fixpoint `{Nominal X} (a b : name) (x : X) : a # x → b # x → ⟨a,b⟩ • x ≡ x.
 Proof.
   intros FA FB; destruct (decide (a = b)); subst.
   - apply perm_action_equal.
-  - destruct FA as [p ? Fp]; destruct FB as [k ? Fk]; 
+  - destruct FA as [p [? Fp]]; destruct FB as [k [? Fk]];
       destruct (decide (p = k)), (decide (k = a)), (decide (k = b)), 
         (decide (p = a)), (decide (p = b)); subst;
           try first [assumption | apply perm_action_equal | rewrite perm_swap; assumption]. 
