theories/Instances/Name.v
@@ -14,18 +14,21 @@ Proof.
     - symmetry; apply swap_perm_app.
 Defined.
 
-Instance name_nominal : Nominal name.
+Instance name_nominal: Nominal name.
 Proof. split; intros; [apply name_perm | apply swap_neither1; apply not_elem_of_singleton]; auto. Qed.
 
-Lemma name_fresh_neq (a b : name) : a # b → a ≠ b.
+Lemma name_fresh_neq (a b: name): a # b → a ≠ b.
 Proof. 
-    intros [c ? cF]; destruct (decide (a = c)); subst.
+    intros [c [? cF]]; destruct (decide (a = c)); subst.
     - apply not_elem_of_singleton; auto.
     - apply swap_neither2 in cF as [[] | []]; subst; auto.
 Qed.  
 
-Definition name_neq_fresh (a b : name) : a ≠ b → a # b.
+Lemma name_neq_fresh (a b: name): a ≠ b → a # b.
 Proof. 
-    intros; constructor 1 with a; 
+    intros; constructor 1 with a; split;
         [unfold support; apply not_elem_of_singleton | apply swap_neither1]; auto. 
-Qed. 
+Qed.
+
+Lemma name_neq_fresh_iff (a b: name): a # b ↔ a ≠ b.
+Proof. split; [apply name_fresh_neq | apply name_neq_fresh]. Qed.
