theories/Nominal.v
@@ -5,12 +5,12 @@ Class Support A := support: A → nameset.
 Instance: Params (@support) 1 := {}.
 
 Section Nominal.
-  Context (X : Type) `{Perm X}.
+  Context (X: Type) `{Perm X}.
 
-  Class Nominal `{Spt : Support X}: Prop := {
+  Class Nominal `{Spt: Support X}: Prop := {
     nperm :> Perm X;
     support_spec : ∀ (x: X) (a b: name),
-        a ∉ (support x) → b ∉ (support x) → ⟨a,b⟩ • x ≡@{X} x
+      a ∉ (support x) → b ∉ (support x) → ⟨a,b⟩ • x ≡@{X} x
 }.
 End Nominal.
 Arguments support_spec {_ PrA _ _ Nmn} : rename.
@@ -21,7 +21,7 @@ Arguments support_spec {_ PrA _ _ Nmn} : rename.
   Lemma lala : (a ∉ support x) → (c ∉ support x) →
     a ≠ b → b ≠ c →
     ⟨ c, a ⟩ • ⟨ a, b ⟩ • x ≡ ⟨ c, b ⟩ • x.
-  Proof. 
+  Proof.
     intros; rewrite (perm_expand c a b).
     + repeat rewrite <- gact_compat. rewrite (support_spec x c a). auto.
     + auto.
